Work on coqdoc for NNRC

coq/NNRC/Lang/NNRC.v
@@ -19,8 +19,7 @@ intermediate language to facilitate code generation for non-functional
 targets. *)
 
 (** NNRC is a thin layer over the core language cNNRC. As cNNRC, NNRC
-  is evaluated within a global (static) environment and local
-  environment. *)
+  is evaluated within a local environment. *)
 
 (** Additional operators in NNRC can be easily expressed in terms of
   the core cNNRC, but are useful for optimization purposes. The main
@@ -52,449 +51,182 @@ Section NNRC.
   Require Import Utils BasicRuntime.
   Require Import cNNRC.
 
-  Section Language.
-    Context {fruntime:foreign_runtime}.
+  Context {fruntime:foreign_runtime}.
+
+  (** * Abstract Syntax *)
+  
+  (** The full abstract syntax for NNRC is already defined in core cNNRC. *)
+
+  Definition nnrc := nnrc.
+
+  (** * Macros *)
+  
+  (** All the additional operators are defined in terms of the core cNNRC. *)
+  
+  Section Macros.
     Context {h:brand_relation_t}.
 
-    (** The AST for NNRC is fully defined in the core NNRC module *)
-    Definition nnrc := nnrc.
-  
-    Section macros.
-      (** e groupby[g,keys] ==
+    (** The following macro defines group-by in terms of existing cNNRC expressions. *)
+
+    (** [e groupby[g,keys] ==
          LET $group0 := e
-         IN { [ g: ]
-                ⊕
-              ♯flatten({ IF ($group3 = π[keys])
-                         THEN {$group3}
-                         ELSE {}
-                       | $group3 ∈ $group0 })
-            | $group2 ∈ ♯distinct({ π[keys]($group1) | $group1 ∈ $group0 }) }
-       *)
-      Definition nnrc_group_by (g:string) (sl:list string) (e:nnrc) : nnrc :=
-        let t0 := "$group0"%string in
-        let t1 := "$group1"%string in
-        let t2 := "$group2"%string in
-        let t3 := "$group3"%string in
-        NNRCLet t0 e
-                (NNRCFor t2
-                         (NNRCUnop ADistinct
-                                   (NNRCFor t1 (NNRCVar t0) (NNRCUnop (ARecProject sl) (NNRCVar t1))))
-                         (NNRCBinop AConcat
-                                    (NNRCUnop (ARec g)
-                                              (NNRCUnop AFlatten
-                                                        (NNRCFor t3 (NNRCVar t0)
-                                                                 (NNRCIf (NNRCBinop AEq (NNRCUnop (ARecProject sl) (NNRCVar t3)) (NNRCVar t2))
-                                                                         (NNRCUnop AColl (NNRCVar t3))
-                                                                         (NNRCConst (dcoll nil))))))
-                                    (NNRCVar t2))).
+         IN { [ g: ♯flatten({ IF ($group3 = π[keys])
+                              THEN {$group3}
+                              ELSE {}
+                              | $group3 ∈ $group0 }) ]
+            | $group2 ∈ ♯distinct({ π[keys]($group1)
+                                  | $group1 ∈ $group0 }) }]
+     *)
+
+    Definition nnrc_group_by (g:string) (sl:list string) (e:nnrc) : nnrc :=
+      let t0 := "$group0"%string in
+      let t1 := "$group1"%string in
+      let t2 := "$group2"%string in
+      let t3 := "$group3"%string in
+      NNRCLet
+        t0 e
+        (NNRCFor t2
+                 (NNRCUnop ADistinct
+                           (NNRCFor t1 (NNRCVar t0) (NNRCUnop (ARecProject sl) (NNRCVar t1))))
+                 (NNRCBinop AConcat
+                            (NNRCUnop (ARec g)
+                                      (NNRCUnop AFlatten
+                                                (NNRCFor t3 (NNRCVar t0)
+                                                         (NNRCIf (NNRCBinop AEq
+                                                                            (NNRCUnop (ARecProject sl)
+                                                                                      (NNRCVar t3))
+                                                                            (NNRCVar t2))
+                                                                       (NNRCUnop AColl (NNRCVar t3))
+                                                                       (NNRCConst (dcoll nil))))))
+                            (NNRCVar t2))).
+
+    (** This definition is equivalent to a nested evaluation group by algorithm. *)
     
-      Lemma nnrc_group_by_correct env
-            (g:string) (sl:list string)
-            (e:nnrc)
-            (incoll outcoll:list data):
-        nnrc_core_eval h env e = Some (dcoll incoll) ->
-        group_by_nested_eval_table g sl incoll = Some outcoll -> 
-        nnrc_core_eval h env (nnrc_group_by g sl e) = Some (dcoll outcoll).
-      Proof.
-        intros.
-        unfold nnrc_group_by; simpl.
-        rewrite H; simpl; clear H.
-        apply (group_by_table_correct g sl incoll outcoll H0).
-      Qed.
+    Lemma nnrc_group_by_correct env
+          (g:string) (sl:list string)
+          (e:nnrc)
+          (incoll outcoll:list data):
+      nnrc_core_eval h env e = Some (dcoll incoll) ->
+      group_by_nested_eval_table g sl incoll = Some outcoll -> 
+      nnrc_core_eval h env (nnrc_group_by g sl e) = Some (dcoll outcoll).
+    Proof.
+      intros.
+      unfold nnrc_group_by; simpl.
+      rewrite H; simpl; clear H.
+      apply (group_by_table_correct g sl incoll outcoll H0).
+    Qed.
 
-      Definition nnrc_group_by_from_nraenv (vid venv:var) (g:string) (sl:list string) (e:nnrc) :=
-        (NNRCLet (fresh_var "tappe$" (vid :: venv :: nil))
-                 (NNRCUnop (ARec "$pregroup") e)
-                 (NNRCFor
-                    (fresh_var "tmap$"
-                               (vid :: fresh_var "tappe$" (vid :: venv :: nil) :: nil))
-                    (NNRCUnop ADistinct
-                              (NNRCFor
-                                 (fresh_var "tmap$"
-                                            (vid :: fresh_var "tappe$" (vid :: venv :: nil) :: nil))
-                                 (NNRCUnop (ADot "$pregroup")
-                                           (NNRCVar (fresh_var "tappe$" (vid :: venv :: nil))))
-                                 (NNRCUnop (ARecProject sl)
-                                           (NNRCVar
-                                              (fresh_var "tmap$"
-                                                         (vid
-                                                            :: fresh_var "tappe$" (vid :: venv :: nil)
-                                                            :: nil))))))
-                    (NNRCBinop AConcat
-                               (NNRCUnop (ARec g)
-                                         (NNRCLet
-                                            (fresh_var "tappe$"
-                                                       (fresh_var "tmap$"
-                                                                  (vid
-                                                                     :: fresh_var "tappe$" (vid :: venv :: nil)
-                                                                     :: nil)
-                                                                  :: fresh_var "tappe$" (vid :: venv :: nil) :: nil))
-                                            (NNRCBinop AConcat
-                                                       (NNRCUnop (ARec "$key")
-                                                                 (NNRCVar
-                                                                    (fresh_var "tmap$"
-                                                                               (vid
-                                                                                  :: fresh_var "tappe$" (vid :: venv :: nil)
-                                                                                  :: nil))))
-                                                       (NNRCVar (fresh_var "tappe$" (vid :: venv :: nil))))
-                                            (NNRCUnop AFlatten
-                                                      (NNRCFor
-                                                         (fresh_var "tsel$"
-                                                                    (fresh_var "tmap$"
-                                                                               (vid
-                                                                                  :: fresh_var "tappe$" (vid :: venv :: nil)
-                                                                                  :: nil)
-                                                                               :: fresh_var "tappe$"
-                                                                               (fresh_var "tmap$"
-                                                                                          (vid
-                                                                                             :: fresh_var "tappe$"
-                                                                                             (vid :: venv :: nil) :: nil)
-                                                                                          :: fresh_var "tappe$"
-                                                                                          (vid :: venv :: nil) :: nil)
-                                                                               :: nil))
-                                                         (NNRCUnop (ADot "$pregroup")
-                                                                   (NNRCVar
-                                                                      (fresh_var "tappe$"
-                                                                                 (fresh_var "tmap$"
-                                                                                            (vid
-                                                                                               :: fresh_var "tappe$"
-                                                                                               (vid :: venv :: nil) :: nil)
-                                                                                            :: fresh_var "tappe$"
-                                                                                            (vid :: venv :: nil) :: nil))))
-                                                         (NNRCIf
-                                                            (NNRCBinop AEq
-                                                                       (NNRCUnop (ARecProject sl)
-                                                                                 (NNRCVar
-                                                                                    (fresh_var "tsel$"
-                                                                                               (fresh_var "tmap$"
-                                                                                                          (vid
-                                                                                                             :: fresh_var "tappe$"
-                                                                                                             (vid :: venv :: nil)
-                                                                                                             :: nil)
-                                                                                                          :: fresh_var "tappe$"
-                                                                                                          (fresh_var "tmap$"
-                                                                                                                     (vid
-                                                                                                                        :: 
-                                                                                                                        fresh_var "tappe$"
-                                                                                                                        (vid :: venv :: nil)
-                                                                                                                        :: nil)
-                                                                                                                     :: 
-                                                                                                                     fresh_var "tappe$"
-                                                                                                                     (vid :: venv :: nil)
-                                                                                                                     :: nil) :: nil))))
-                                                                       (NNRCUnop (ADot "$key")
-                                                                                 (NNRCVar
-                                                                                    (fresh_var "tappe$"
-                                                                                               (fresh_var "tmap$"
-                                                                                                          (vid
-                                                                                                             :: fresh_var "tappe$"
-                                                                                                             (vid :: venv :: nil)
-                                                                                                             :: nil)
-                                                                                                          :: fresh_var "tappe$"
-                                                                                                          (vid :: venv :: nil) :: nil)))))
-                                                            (NNRCUnop AColl
-                                                                      (NNRCVar
-                                                                         (fresh_var "tsel$"
-                                                                                    (fresh_var "tmap$"
-                                                                                               (vid
-                                                                                                  :: fresh_var "tappe$"
-                                                                                                  (vid :: venv :: nil) :: nil)
-                                                                                               :: fresh_var "tappe$"
-                                                                                               (fresh_var "tmap$"
-                                                                                                          (vid
-                                                                                                             :: 
-                                                                                                             fresh_var "tappe$"
-                                                                                                             (vid :: venv :: nil)
-                                                                                                             :: nil)
-                                                                                                          :: fresh_var "tappe$"
-                                                                                                          (vid :: venv :: nil)
-                                                                                                          :: nil) :: nil))))
-                                                            (NNRCConst (dcoll nil)))))))
-                               (NNRCVar
-                                  (fresh_var "tmap$"
-                                             (vid :: fresh_var "tappe$" (vid :: venv :: nil) :: nil)))))).
+  End Macros.
+
+  (** * Evaluation Semantics *)
+
+  Section Semantics.
+    Context {h:brand_relation_t}.
+
+    Fixpoint nnrc_ext_to_nnrc (e:nnrc) : nnrc :=
+      match e with
+      | NNRCVar v => NNRCVar v
+      | NNRCConst d => NNRCConst d
+      | NNRCBinop b e1 e2 =>
+        NNRCBinop b (nnrc_ext_to_nnrc e1) (nnrc_ext_to_nnrc e2)
+      | NNRCUnop u e1 =>
+        NNRCUnop u (nnrc_ext_to_nnrc e1)
+      | NNRCLet v e1 e2 =>
+        NNRCLet v (nnrc_ext_to_nnrc e1) (nnrc_ext_to_nnrc e2)
+      | NNRCFor v e1 e2 =>
+        NNRCFor v (nnrc_ext_to_nnrc e1) (nnrc_ext_to_nnrc e2)
+      | NNRCIf e1 e2 e3 =>
+        NNRCIf (nnrc_ext_to_nnrc e1) (nnrc_ext_to_nnrc e2) (nnrc_ext_to_nnrc e3)
+      | NNRCEither e1 v2 e2 v3 e3 =>
+        NNRCEither (nnrc_ext_to_nnrc e1) v2 (nnrc_ext_to_nnrc e2) v3 (nnrc_ext_to_nnrc e3)
+      | NNRCGroupBy g sl e1 =>
+        nnrc_group_by g sl (nnrc_ext_to_nnrc e1)
+      end.
+
+    Definition nnrc_ext_eval (env:bindings) (e:nnrc) : option data :=
+      nnrc_core_eval h env (nnrc_ext_to_nnrc e).
       
-      Lemma rmap1 sl l :
-        (rmap
-           (fun d1 : data =>
-              match d1 with
-              | dunit => None
-              | dnat _ => None
-              | dbool _ => None
-              | dstring _ => None
-              | dcoll _ => None
-              | drec r => Some (drec (rproject r sl))
-              | dleft _ => None
-              | dright _ => None
-              | dbrand _ _ => None
-              | dforeign _ => None
-              end) l) =
-        (rmap
-           (fun d1 : data =>
-              olift
-                (fun d0 : data =>
-                   match d0 with
-                   | dunit => None
-                   | dnat _ => None
-                   | dbool _ => None
-                   | dstring _ => None
-                   | dcoll _ => None
-                   | drec r => Some (drec (rproject r sl))
-                   | dleft _ => None
-                   | dright _ => None
-                   | dbrand _ _ => None
-                   | dforeign _ => None
-                   end) (Some d1)) l).
-      Proof.
-        apply rmap_ext; intros.
-        reflexivity.
-      Qed.
+    Remark nnrc_ext_to_nnrc_eq (e:nnrc):
+      forall env,
+        nnrc_ext_eval env e = nnrc_core_eval h env (nnrc_ext_to_nnrc e).
+    Proof.
+      intros; reflexivity.
+    Qed.
 
-      Lemma pick_fresh_distinct_second v v1 v2 rest:
-        exists v3,
-          v3 = (fresh_var v (v1 :: v2 :: rest)) /\
-          v2 <> v3.
-      Proof.
-        exists (fresh_var v (v1 :: v2 :: rest)).
-        split;[reflexivity| ].
-        apply fresh_var_fresh2.
-      Qed.
-
-      Lemma build_group_ext (x:data) (o1 o2:option data) :
-        o1 = o2 ->
-        match o1 with
-        | Some dunit => None
-        | Some (dnat _) => None
-        | Some (dbool _) => None
-        | Some (dstring _) => None
-        | Some (dcoll _) => None
-        | Some (drec r1) =>
-          match x with
-          | dunit => None
-          | dnat _ => None
-          | dbool _ => None
-          | dstring _ => None
-          | dcoll _ => None
-          | drec r2 => Some (drec (rec_sort (r1 ++ r2)))
-          | dleft _ => None
-          | dright _ => None
-          | dbrand _ _ => None
-          | dforeign _ => None
-          end
-        | Some (dleft _) => None
-        | Some (dright _) => None
-        | Some (dbrand _ _) => None
-        | Some (dforeign _) => None
-        | None => None
-        end =
-        match o2 with
-        | Some dunit => None
-        | Some (dnat _) => None
-        | Some (dbool _) => None
-        | Some (dstring _) => None
-        | Some (dcoll _) => None
-        | Some (drec r1) =>
-          match x with
-          | dunit => None
-          | dnat _ => None
-          | dbool _ => None
-          | dstring _ => None
-          | dcoll _ => None
-          | drec r2 => Some (drec (rec_sort (r1 ++ r2)))
-          | dleft _ => None
-          | dright _ => None
-          | dbrand _ _ => None
-          | dforeign _ => None
-          end
-        | Some (dleft _) => None
-        | Some (dright _) => None
-        | Some (dbrand _ _) => None
-        | Some (dforeign _) => None
-        | None => None
-        end.
-      Proof.
-        intros Hinput; rewrite Hinput; clear Hinput.
-        reflexivity.
-      Qed.
-
-      Lemma nnrc_core_eval_group_by_eq env (g:string) (sl:list string) (e1 e2:nnrc):
-        nnrc_core_eval h env e1 = nnrc_core_eval h env e2 ->
-        forall vid venv,
-          nnrc_core_eval h env (nnrc_group_by g sl e1)
-          = nnrc_core_eval h env (nnrc_group_by_from_nraenv vid venv g sl e2).
-      Proof.
-        intro Heval; intros.
-        unfold nnrc_group_by, nnrc_group_by_from_nraenv.
-        Opaque fresh_var.
-        simpl.
-        rewrite <- Heval; clear Heval.
-        destruct (nnrc_core_eval h env e1); [|reflexivity]; simpl; clear e1 e2.
-        generalize (fresh_var "tappe$" (vid :: venv :: nil)); intro v0.
-        destruct (equiv_dec v0 v0); try congruence.
-        destruct d; try reflexivity; simpl.
-        generalize (pick_fresh_distinct_second "tmap$" vid v0 nil); intros Hpick.
-        elim Hpick; clear Hpick; intro v1; intros.
-        elim H; clear H; intros.
-        assert ((fresh_var
-                   (String
-                      (Ascii.Ascii false false true false true true true false)
-                      (String
-                         (Ascii.Ascii true false true true false true true false)
-                         (String
-                            (Ascii.Ascii true false false false false true true
-                                         false)
-                            (String
-                               (Ascii.Ascii false false false false true true true
-                                            false)
-                               (String
-                                  (Ascii.Ascii false false true false false true
-                                               false false) EmptyString)))))
-                   (@cons string vid (@cons string v0 (@nil string)))) =
-                fresh_var "tmap$" (vid :: v0 :: nil)).
-        reflexivity.
-        rewrite H1 in H; clear H1.
-        rewrite <- H; clear H.
-        destruct (equiv_dec v1 v1); try congruence; clear e0.
-        rewrite <- rmap1.
-        destruct (rmap
-                    (fun d1 : data =>
-                       match d1 with
-                       | dunit => None
-                       | dnat _ => None
-                       | dbool _ => None
-                       | dstring _ => None
-                       | dcoll _ => None
-                       | drec r => Some (drec (rproject r sl))
-                       | dleft _ => None
-                       | dright _ => None
-                       | dbrand _ _ => None
-                       | dforeign _ => None
-                       end) l); try reflexivity; simpl.
-        f_equal.
-        apply rmap_ext; intros. simpl.
-        destruct (equiv_dec v0 v1); try congruence; clear c; simpl.
-        destruct (equiv_dec (fresh_var "tappe$" (v1 :: v0 :: nil))
-                            (fresh_var "tappe$" (v1 :: v0 :: nil))); try congruence;
-          simpl; clear e0.
-        unfold olift2.
-        apply build_group_ext.
-        f_equal.
-        f_equal.
-        f_equal.
-        apply rmap_ext; intros.
-        unfold olift.
-        generalize (fresh_var "tappe$" (v1 :: v0 :: nil)); intros v2.
-        destruct (equiv_dec (fresh_var "tsel$" (v1 :: v2 :: nil))
-                            (fresh_var "tsel$" (v1 :: v2 :: nil))); try congruence;
-          clear e0; simpl.
-        generalize (pick_fresh_distinct_second "tsel$" v1 v2 nil); intros Hpick.
-        elim Hpick; clear Hpick; intro v3; intros.
-        elim H2; clear H2; intros.
-        rewrite <- H2; clear H2.
-        destruct (equiv_dec v2 v3); try congruence; clear c.
-        simpl.
-        reflexivity.
-      Qed.
-
-    End macros.
-
-    Section translation.
-      Fixpoint nnrc_ext_to_nnrc (e:nnrc) : nnrc :=
-        match e with
-        | NNRCVar v => NNRCVar v
-        | NNRCConst d => NNRCConst d
-        | NNRCBinop b e1 e2 =>
-          NNRCBinop b (nnrc_ext_to_nnrc e1) (nnrc_ext_to_nnrc e2)
-        | NNRCUnop u e1 =>
-          NNRCUnop u (nnrc_ext_to_nnrc e1)
-        | NNRCLet v e1 e2 =>
-          NNRCLet v (nnrc_ext_to_nnrc e1) (nnrc_ext_to_nnrc e2)
-        | NNRCFor v e1 e2 =>
-          NNRCFor v (nnrc_ext_to_nnrc e1) (nnrc_ext_to_nnrc e2)
-        | NNRCIf e1 e2 e3 =>
-          NNRCIf (nnrc_ext_to_nnrc e1) (nnrc_ext_to_nnrc e2) (nnrc_ext_to_nnrc e3)
-        | NNRCEither e1 v2 e2 v3 e3 =>
-          NNRCEither (nnrc_ext_to_nnrc e1) v2 (nnrc_ext_to_nnrc e2) v3 (nnrc_ext_to_nnrc e3)
-        | NNRCGroupBy g sl e1 =>
-          nnrc_group_by g sl (nnrc_ext_to_nnrc e1)
-        end.
-
-      Lemma nnrc_ext_to_nnrc_is_core (e:nnrc) :
-        nnrcIsCore (nnrc_ext_to_nnrc e).
-      Proof.
-        induction e; intros; simpl in *; auto.
-        repeat (split; auto).
-      Qed.
+    (** Since we rely on cNNRC abstract syntax for the whole NNRC, it is important to check that translating to the core does not reuse the additional operations only present in NNRC. *)
     
-      Lemma core_nnrc_to_nnrc_ext_id (e:nnrc) :
-        nnrcIsCore e ->
-        (nnrc_ext_to_nnrc e) = e.
-      Proof.
-        intros.
-        induction e; simpl in *.
-        - reflexivity.
-        - reflexivity.
-        - elim H; intros.
-          rewrite IHe1; auto; rewrite IHe2; auto.
-        - rewrite IHe; auto.
-        - elim H; intros.
-          rewrite IHe1; auto; rewrite IHe2; auto.
-        - elim H; intros.
-          rewrite IHe1; auto; rewrite IHe2; auto.
-        - elim H; intros.
-          elim H1; intros.
-          rewrite IHe1; auto; rewrite IHe2; auto; rewrite IHe3; auto.
-        - elim H; intros.
-          elim H1; intros.
-          rewrite IHe1; auto; rewrite IHe2; auto; rewrite IHe3; auto.
-        - contradiction. (* GroupBy case *)
-      Qed.
+    Lemma nnrc_ext_to_nnrc_is_core (e:nnrc) :
+      nnrcIsCore (nnrc_ext_to_nnrc e).
+    Proof.
+      induction e; intros; simpl in *; auto.
+      repeat (split; auto).
+    Qed.
 
-      Lemma core_nnrc_to_nnrc_ext_idempotent (e1 e2:nnrc) :
-        e1 = nnrc_ext_to_nnrc e2 ->
-        nnrc_ext_to_nnrc e1 = e1.
-      Proof.
-        intros.
-        apply core_nnrc_to_nnrc_ext_id.
-        rewrite H.
-        apply nnrc_ext_to_nnrc_is_core.
-      Qed.
-
-      Corollary core_nnrc_to_nnrc_ext_idempotent_corr (e:nnrc) :
-        nnrc_ext_to_nnrc (nnrc_ext_to_nnrc e) = (nnrc_ext_to_nnrc e).
-      Proof.
-        apply (core_nnrc_to_nnrc_ext_idempotent _ e).
-        reflexivity.
-      Qed.
+    (** The following function effectively returns an abstract syntax
+    tree with the right type for cNNRC. *)
     
-    End translation.
+    Program Definition nnrc_to_nnrc_core (e:nnrc) : nnrc_core :=
+      nnrc_ext_to_nnrc e.
+    Next Obligation.
+      apply nnrc_ext_to_nnrc_is_core.
+    Defined.
 
-    Section semantics.
-      (** Semantics of NNRCExt *)
-      
-      Definition nnrc_ext_eval (env:bindings) (e:nnrc) : option data :=
-        nnrc_core_eval h env (nnrc_ext_to_nnrc e).
-      
-      Remark nnrc_ext_to_nnrc_eq (e:nnrc):
-        forall env,
-          nnrc_ext_eval env e = nnrc_core_eval h env (nnrc_ext_to_nnrc e).
-      Proof.
-        intros; reflexivity.
-      Qed.
-      
-      Remark nnrc_to_nnrc_ext_eq (e:nnrc):
-        nnrcIsCore e ->
-        forall env,
-          nnrc_core_eval h env e = nnrc_ext_eval env e.
-      Proof.
-        intros.
-        unfold nnrc_ext_eval.
-        rewrite core_nnrc_to_nnrc_ext_id.
-        reflexivity.
-        assumption.
-      Qed.
-      
-    (* we are only sensitive to the environment up to lookup *)
+    (** Additional properties of the translation from NNRC to cNNRC. *)
+    
+    Lemma core_nnrc_to_nnrc_ext_id (e:nnrc) :
+      nnrcIsCore e ->
+      (nnrc_ext_to_nnrc e) = e.
+    Proof.
+      intros.
+      induction e; simpl in *.
+      - reflexivity.
+      - reflexivity.
+      - elim H; intros.
+        rewrite IHe1; auto; rewrite IHe2; auto.
+      - rewrite IHe; auto.
+      - elim H; intros.
+        rewrite IHe1; auto; rewrite IHe2; auto.
+      - elim H; intros.
+        rewrite IHe1; auto; rewrite IHe2; auto.
+      - elim H; intros.
+        elim H1; intros.
+        rewrite IHe1; auto; rewrite IHe2; auto; rewrite IHe3; auto.
+      - elim H; intros.
+        elim H1; intros.
+        rewrite IHe1; auto; rewrite IHe2; auto; rewrite IHe3; auto.
+      - contradiction. (* GroupBy case *)
+    Qed.
+    
+    Lemma core_nnrc_to_nnrc_ext_idempotent (e1 e2:nnrc) :
+      e1 = nnrc_ext_to_nnrc e2 ->
+      nnrc_ext_to_nnrc e1 = e1.
+    Proof.
+      intros.
+      apply core_nnrc_to_nnrc_ext_id.
+      rewrite H.
+      apply nnrc_ext_to_nnrc_is_core.
+    Qed.
+
+    Corollary core_nnrc_to_nnrc_ext_idempotent_corr (e:nnrc) :
+      nnrc_ext_to_nnrc (nnrc_ext_to_nnrc e) = (nnrc_ext_to_nnrc e).
+    Proof.
+      apply (core_nnrc_to_nnrc_ext_idempotent _ e).
+      reflexivity.
+    Qed.
+
+    Remark nnrc_to_nnrc_ext_eq (e:nnrc):
+      nnrcIsCore e ->
+      forall env,
+        nnrc_core_eval h env e = nnrc_ext_eval env e.
+    Proof.
+      intros.
+      unfold nnrc_ext_eval.
+      rewrite core_nnrc_to_nnrc_ext_id.
+      reflexivity.
+      assumption.
+    Qed.
+    
+    (** we are only sensitive to the environment up to lookup *)
     Global Instance nnrc_ext_eval_lookup_equiv_prop :
       Proper (lookup_equiv ==> eq ==> eq) nnrc_ext_eval.
     Proof.
@@ -506,9 +238,14 @@ Section NNRC.
       reflexivity.
     Qed.
     
-  End semantics.
+  End Semantics.
 
-  Section prop.
+  (** * Additional Properties *)
+
+  (** Most of the following properties are useful for shadowing and variable substitution on the full NNRC. *)
+  
+  Section Properties.
+    Context {h:brand_relation_t}.
     Require Import cNNRCShadow.
     
     Lemma nnrc_ext_to_nnrc_free_vars_same e:
@@ -620,7 +357,7 @@ Section NNRC.
         destruct (equiv_dec "$group2"%string v1); try congruence; try reflexivity.
         destruct (equiv_dec "$group3"%string v1); try congruence; try reflexivity.
     Qed.
-        
+
     Lemma nnrc_ext_to_nnrc_rename_lazy_comm e v1 v2:
       nnrc_rename_lazy (nnrc_ext_to_nnrc e) v1 v2 =
       nnrc_ext_to_nnrc (nnrc_rename_lazy e v1 v2).
@@ -680,7 +417,7 @@ Section NNRC.
         destruct (equiv_dec "$group3"%string v1); try congruence; try reflexivity.
     Qed.
 
-    (* unshadow properties for extended NNRC *)
+    (** Unshadow properties for the full NNRC. *)
     Lemma unshadow_over_nnrc_ext_idem sep renamer avoid e:
       (nnrc_ext_to_nnrc (unshadow sep renamer avoid (nnrc_ext_to_nnrc e))) =
       (unshadow sep renamer avoid (nnrc_ext_to_nnrc e)).
@@ -695,8 +432,8 @@ Section NNRC.
     Lemma nnrc_ext_eval_cons_subst e env v x v' :
       ~ (In v' (nnrc_free_vars e)) ->
       ~ (In v' (nnrc_bound_vars e)) ->
-      nnrc_ext_eval ((v',x)::env) (nnrc_subst e v (NNRCVar v')) = 
-      nnrc_ext_eval ((v,x)::env) e.
+      @nnrc_ext_eval h ((v',x)::env) (nnrc_subst e v (NNRCVar v')) = 
+      @nnrc_ext_eval h ((v,x)::env) e.
     Proof.
       revert env v x v'.
       nnrc_cases (induction e) Case; simpl; unfold equiv_dec;
@@ -782,96 +519,18 @@ Section NNRC.
         reflexivity.
     Qed.
 
-    Definition unnest_from_nraenv vid venv a b n1 := 
-      (NNRCFor (fresh_var "tmap$" (vid :: venv :: nil))
-               (NNRCUnop AFlatten
-                         (NNRCFor (fresh_var "tmc$" (vid :: venv :: nil))
-                                  n1
-                                  (NNRCFor
-                                     (fresh_var "tmc$" (fresh_var "tmc$" (vid :: venv :: nil) :: vid :: venv :: nil))
-                                     (NNRCFor (fresh_var "tmap$" (vid :: venv :: nil))
-                                              (NNRCUnop (ADot a) (NNRCVar (fresh_var "tmc$" (vid :: venv :: nil))))
-                                              (NNRCUnop (ARec b) (NNRCVar (fresh_var "tmap$" (vid :: venv :: nil)))))
-                                     (NNRCBinop AConcat (NNRCVar (fresh_var "tmc$" (vid :: venv :: nil)))
-                                                (NNRCVar
-                                                   (fresh_var "tmc$"
-                                                              (fresh_var "tmc$" (vid :: venv :: nil) :: vid :: venv :: nil)))))))
-               (NNRCUnop (ARecRemove a) (NNRCVar (fresh_var "tmap$" (vid :: venv :: nil))))).
+  End Properties.
 
-    Definition unnest_from_nraenv_core vid venv a b n1 :=
-      (NNRCFor (fresh_var "tmap$" (vid :: venv :: nil))
-               (NNRCUnop AFlatten
-                         (NNRCFor (fresh_var "tmc$" (vid :: venv :: nil))
-                                  n1
-                                  (NNRCFor
-                                     (fresh_var "tmc$" (fresh_var "tmc$" (vid :: venv :: nil) :: vid :: venv :: nil))
-                                     (NNRCFor
-                                        (fresh_var "tmap$" (fresh_var "tmc$" (vid :: venv :: nil) :: venv :: nil))
-                                        (NNRCUnop (ADot a) (NNRCVar (fresh_var "tmc$" (vid :: venv :: nil))))
-                                        (NNRCUnop (ARec b)
-                                                  (NNRCVar
-                                                     (fresh_var "tmap$"
-                                                                (fresh_var "tmc$" (vid :: venv :: nil) :: venv :: nil)))))
-                                     (NNRCBinop AConcat (NNRCVar (fresh_var "tmc$" (vid :: venv :: nil)))
-                                                (NNRCVar
-                                                   (fresh_var "tmc$"
-                                                              (fresh_var "tmc$" (vid :: venv :: nil) :: vid :: venv :: nil)))))))
-               (NNRCUnop (ARecRemove a) (NNRCVar (fresh_var "tmap$" (vid :: venv :: nil))))).
-
-    Lemma unnest_from_nraenv_and_nraenv_core_eq vid venv env a b op1 op1' :
-      nnrc_core_eval h env op1 = nnrc_core_eval h env op1' ->
-      nnrc_core_eval h env (unnest_from_nraenv vid venv a b op1) =
-      nnrc_core_eval h env (unnest_from_nraenv_core vid venv a b op1').
-    Proof.
-      intros Hind.
-      Opaque fresh_var.
-      simpl.
-      rewrite Hind; clear Hind.
-      destruct (nnrc_core_eval h env op1'); try reflexivity; simpl.
-      destruct d; try reflexivity; simpl.
-      destruct (equiv_dec (fresh_var "tmap$" (vid :: venv :: nil))
-                          (fresh_var "tmap$" (vid :: venv :: nil))); try congruence.
-      destruct (equiv_dec (fresh_var "tmc$" (vid :: venv :: nil))
-                          (fresh_var "tmc$" (vid :: venv :: nil))); try congruence.
-      simpl in *.
-      destruct (equiv_dec
-                  (fresh_var "tmc$"
-                             (fresh_var "tmc$" (vid :: venv :: nil) :: vid :: venv :: nil))
-                  (fresh_var "tmc$"
-                             (fresh_var "tmc$" (vid :: venv :: nil) :: vid :: venv :: nil)));
-        try congruence; simpl.
-      destruct (equiv_dec
-                  (fresh_var "tmap$"
-                             (fresh_var "tmc$" (vid :: venv :: nil) :: venv :: nil))
-                  (fresh_var "tmap$"
-                             (fresh_var "tmc$" (vid :: venv :: nil) :: venv :: nil))); try congruence; simpl in *.
-      destruct (equiv_dec (fresh_var "tmc$" (vid :: venv :: nil))
-                          (fresh_var "tmc$"
-                                     (fresh_var "tmc$" (vid :: venv :: nil)
-                                                :: vid :: venv :: nil))). auto.
-      clear e e0 e1 e2 c.
-      f_equal.
-      induction l; [reflexivity| ]; simpl.
-      destruct a0; try reflexivity.
-    Qed.
+  (** * Toplevel *)
   
-  End prop.
+  (** Top-level evaluation is used externally by the Q*cert
+  compiler. It takes an NNRC expression and a global environment as
+  input. *)
 
-  Section core.
-    Program Definition nnrc_to_nnrc_core (e:nnrc) : nnrc_core :=
-      nnrc_ext_to_nnrc e.
-    Next Obligation.
-      apply nnrc_ext_to_nnrc_is_core.
-    Defined.
-
-  End core.
-  
-  End Language.
   Section Top.
-    Context {fruntime:foreign_runtime}.
     Context (h:brand_relation_t).
     Definition nnrc_eval_top (q:nnrc) (cenv:bindings) : option data :=
-      @nnrc_ext_eval _ h (rec_sort (mkConstants cenv)) q.
+      @nnrc_ext_eval h (rec_sort (mkConstants cenv)) q.
   End Top.
   
 End NNRC.
