coq/NNRC/Lang/NNRCSugar.v
@@ -1,0 +1,385 @@
+(*
+ * Copyright 2015-2016 IBM Corporation
+ *
+ * Licensed under the Apache License, Version 2.0 (the "License");
+ * you may not use this file except in compliance with the License.
+ * You may obtain a copy of the License at
+ *
+ * http://www.apache.org/licenses/LICENSE-2.0
+ *
+ * Unless required by applicable law or agreed to in writing, software
+ * distributed under the License is distributed on an "AS IS" BASIS,
+ * WITHOUT WARRANTIES OR CONDITIONS OF ANY KIND, either express or implied.
+ * See the License for the specific language governing permissions and
+ * limitations under the License.
+ *)
+
+(** This module contains some additional properties for extended operators in NNRC. Some of those are notably useful later on for proving translations from NRAEnv. *)
+
+Section NNRCSugar.
+
+  Require Import String.
+  Require Import List.
+  Require Import Arith.
+  Require Import EquivDec.
+  Require Import Morphisms.
+  Require Import Arith.
+  Require Import Max.
+  Require Import Bool.
+  Require Import Peano_dec.
+  Require Import EquivDec.
+  Require Import Decidable.
+  Require Import Utils.
+  Require Import BasicRuntime.
+  Require Import cNNRC.
+  Require Import NNRC.
+
+  Context {fruntime:foreign_runtime}.
+  Context {h:brand_relation_t}.
+
+  (** * Group By *)
+
+  (** This is an alternative macro for group by. This is used as a scafolding to prove translation from the GroupBy in NRAEnv to the one in NNRC correct. *)
+  
+  Definition nnrc_group_by_from_nraenv (vid venv:var) (g:string) (sl:list string) (e:nnrc) :=
+    (NNRCLet (fresh_var "tappe$" (vid :: venv :: nil))
+             (NNRCUnop (ARec "$pregroup") e)
+             (NNRCFor
+                (fresh_var "tmap$"
+                           (vid :: fresh_var "tappe$" (vid :: venv :: nil) :: nil))
+                (NNRCUnop ADistinct
+                          (NNRCFor
+                             (fresh_var "tmap$"
+                                        (vid :: fresh_var "tappe$" (vid :: venv :: nil) :: nil))
+                             (NNRCUnop (ADot "$pregroup")
+                                       (NNRCVar (fresh_var "tappe$" (vid :: venv :: nil))))
+                             (NNRCUnop (ARecProject sl)
+                                       (NNRCVar
+                                          (fresh_var "tmap$"
+                                                     (vid
+                                                        :: fresh_var "tappe$" (vid :: venv :: nil)
+                                                        :: nil))))))
+                (NNRCBinop AConcat
+                           (NNRCUnop (ARec g)
+                                     (NNRCLet
+                                        (fresh_var "tappe$"
+                                                   (fresh_var "tmap$"
+                                                              (vid
+                                                                 :: fresh_var "tappe$" (vid :: venv :: nil)
+                                                                 :: nil)
+                                                              :: fresh_var "tappe$" (vid :: venv :: nil) :: nil))
+                                        (NNRCBinop AConcat
+                                                   (NNRCUnop (ARec "$key")
+                                                             (NNRCVar
+                                                                (fresh_var "tmap$"
+                                                                           (vid
+                                                                              :: fresh_var "tappe$" (vid :: venv :: nil)
+                                                                              :: nil))))
+                                                   (NNRCVar (fresh_var "tappe$" (vid :: venv :: nil))))
+                                        (NNRCUnop AFlatten
+                                                  (NNRCFor
+                                                     (fresh_var "tsel$"
+                                                                (fresh_var "tmap$"
+                                                                           (vid
+                                                                              :: fresh_var "tappe$" (vid :: venv :: nil)
+                                                                              :: nil)
+                                                                           :: fresh_var "tappe$"
+                                                                           (fresh_var "tmap$"
+                                                                                      (vid
+                                                                                         :: fresh_var "tappe$"
+                                                                                         (vid :: venv :: nil) :: nil)
+                                                                                      :: fresh_var "tappe$"
+                                                                                      (vid :: venv :: nil) :: nil)
+                                                                           :: nil))
+                                                     (NNRCUnop (ADot "$pregroup")
+                                                               (NNRCVar
+                                                                  (fresh_var "tappe$"
+                                                                             (fresh_var "tmap$"
+                                                                                        (vid
+                                                                                           :: fresh_var "tappe$"
+                                                                                           (vid :: venv :: nil) :: nil)
+                                                                                        :: fresh_var "tappe$"
+                                                                                        (vid :: venv :: nil) :: nil))))
+                                                     (NNRCIf
+                                                        (NNRCBinop AEq
+                                                                   (NNRCUnop (ARecProject sl)
+                                                                             (NNRCVar
+                                                                                (fresh_var "tsel$"
+                                                                                           (fresh_var "tmap$"
+                                                                                                      (vid
+                                                                                                         :: fresh_var "tappe$"
+                                                                                                         (vid :: venv :: nil)
+                                                                                                         :: nil)
+                                                                                                      :: fresh_var "tappe$"
+                                                                                                      (fresh_var "tmap$"
+                                                                                                                 (vid
+                                                                                                                    :: 
+                                                                                                                    fresh_var "tappe$"
+                                                                                                                    (vid :: venv :: nil)
+                                                                                                                    :: nil)
+                                                                                                                 :: 
+                                                                                                                 fresh_var "tappe$"
+                                                                                                                 (vid :: venv :: nil)
+                                                                                                                 :: nil) :: nil))))
+                                                                   (NNRCUnop (ADot "$key")
+                                                                             (NNRCVar
+                                                                                (fresh_var "tappe$"
+                                                                                           (fresh_var "tmap$"
+                                                                                                      (vid
+                                                                                                         :: fresh_var "tappe$"
+                                                                                                         (vid :: venv :: nil)
+                                                                                                         :: nil)
+                                                                                                      :: fresh_var "tappe$"
+                                                                                                      (vid :: venv :: nil) :: nil)))))
+                                                        (NNRCUnop AColl
+                                                                  (NNRCVar
+                                                                     (fresh_var "tsel$"
+                                                                                (fresh_var "tmap$"
+                                                                                           (vid
+                                                                                              :: fresh_var "tappe$"
+                                                                                              (vid :: venv :: nil) :: nil)
+                                                                                           :: fresh_var "tappe$"
+                                                                                           (fresh_var "tmap$"
+                                                                                                      (vid
+                                                                                                         :: 
+                                                                                                         fresh_var "tappe$"
+                                                                                                         (vid :: venv :: nil)
+                                                                                                         :: nil)
+                                                                                                      :: fresh_var "tappe$"
+                                                                                                      (vid :: venv :: nil)
+                                                                                                      :: nil) :: nil))))
+                                                        (NNRCConst (dcoll nil)))))))
+                           (NNRCVar
+                              (fresh_var "tmap$"
+                                         (vid :: fresh_var "tappe$" (vid :: venv :: nil) :: nil)))))).
+  
+  Lemma pick_fresh_distinct_second v v1 v2 rest:
+    exists v3,
+      v3 = (fresh_var v (v1 :: v2 :: rest)) /\
+      v2 <> v3.
+  Proof.
+    exists (fresh_var v (v1 :: v2 :: rest)).
+    split;[reflexivity| ].
+    apply fresh_var_fresh2.
+  Qed.
+
+  Lemma build_group_ext (x:data) (o1 o2:option data) :
+    o1 = o2 ->
+    match o1 with
+    | Some dunit => None
+    | Some (dnat _) => None
+    | Some (dbool _) => None
+    | Some (dstring _) => None
+    | Some (dcoll _) => None
+    | Some (drec r1) =>
+      match x with
+      | dunit => None
+      | dnat _ => None
+      | dbool _ => None
+      | dstring _ => None
+      | dcoll _ => None
+      | drec r2 => Some (drec (rec_sort (r1 ++ r2)))
+      | dleft _ => None
+      | dright _ => None
+      | dbrand _ _ => None
+      | dforeign _ => None
+      end
+    | Some (dleft _) => None
+    | Some (dright _) => None
+    | Some (dbrand _ _) => None
+    | Some (dforeign _) => None
+    | None => None
+    end =
+    match o2 with
+    | Some dunit => None
+    | Some (dnat _) => None
+    | Some (dbool _) => None
+    | Some (dstring _) => None
+    | Some (dcoll _) => None
+    | Some (drec r1) =>
+      match x with
+      | dunit => None
+      | dnat _ => None
+      | dbool _ => None
+      | dstring _ => None
+      | dcoll _ => None
+      | drec r2 => Some (drec (rec_sort (r1 ++ r2)))
+      | dleft _ => None
+      | dright _ => None
+      | dbrand _ _ => None
+      | dforeign _ => None
+      end
+    | Some (dleft _) => None
+    | Some (dright _) => None
+    | Some (dbrand _ _) => None
+    | Some (dforeign _) => None
+    | None => None
+    end.
+  Proof.
+    intros Hinput; rewrite Hinput; clear Hinput.
+    reflexivity.
+  Qed.
+
+  (** The following states that the principal definition for group by and this alternative are equivalent. *)
+  
+  Lemma nnrc_core_eval_group_by_eq env (g:string) (sl:list string) (e1 e2:nnrc):
+    nnrc_core_eval h env e1 = nnrc_core_eval h env e2 ->
+    forall vid venv,
+      nnrc_core_eval h env (nnrc_group_by g sl e1)
+      = nnrc_core_eval h env (nnrc_group_by_from_nraenv vid venv g sl e2).
+  Proof.
+    intro Heval; intros.
+    unfold nnrc_group_by, nnrc_group_by_from_nraenv.
+    Opaque fresh_var.
+    simpl.
+    rewrite <- Heval; clear Heval.
+    destruct (nnrc_core_eval h env e1); [|reflexivity]; simpl; clear e1 e2.
+    generalize (fresh_var "tappe$" (vid :: venv :: nil)); intro v0.
+    destruct (equiv_dec v0 v0); try congruence.
+    destruct d; try reflexivity; simpl.
+    generalize (pick_fresh_distinct_second "tmap$" vid v0 nil); intros Hpick.
+    elim Hpick; clear Hpick; intro v1; intros.
+    elim H; clear H; intros.
+    assert ((fresh_var
+               (String
+                  (Ascii.Ascii false false true false true true true false)
+                  (String
+                     (Ascii.Ascii true false true true false true true false)
+                     (String
+                        (Ascii.Ascii true false false false false true true
+                                     false)
+                        (String
+                           (Ascii.Ascii false false false false true true true
+                                        false)
+                           (String
+                              (Ascii.Ascii false false true false false true
+                                           false false) EmptyString)))))
+               (@cons string vid (@cons string v0 (@nil string)))) =
+            fresh_var "tmap$" (vid :: v0 :: nil)).
+    reflexivity.
+    rewrite H1 in H; clear H1.
+    rewrite <- H; clear H.
+    destruct (equiv_dec v1 v1); try congruence; clear e0.
+    rewrite <- rmap_with_rproject.
+    destruct (rmap
+                (fun d1 : data =>
+                   match d1 with
+                   | dunit => None
+                   | dnat _ => None
+                   | dbool _ => None
+                   | dstring _ => None
+                   | dcoll _ => None
+                   | drec r => Some (drec (rproject r sl))
+                   | dleft _ => None
+                   | dright _ => None
+                   | dbrand _ _ => None
+                   | dforeign _ => None
+                   end) l); try reflexivity; simpl.
+    f_equal.
+    apply rmap_ext; intros. simpl.
+    destruct (equiv_dec v0 v1); try congruence; clear c; simpl.
+    destruct (equiv_dec (fresh_var "tappe$" (v1 :: v0 :: nil))
+                        (fresh_var "tappe$" (v1 :: v0 :: nil))); try congruence;
+      simpl; clear e0.
+    unfold olift2.
+    apply build_group_ext.
+    f_equal.
+    f_equal.
+    f_equal.
+    apply rmap_ext; intros.
+    unfold olift.
+    generalize (fresh_var "tappe$" (v1 :: v0 :: nil)); intros v2.
+    destruct (equiv_dec (fresh_var "tsel$" (v1 :: v2 :: nil))
+                        (fresh_var "tsel$" (v1 :: v2 :: nil))); try congruence;
+      clear e0; simpl.
+    generalize (pick_fresh_distinct_second "tsel$" v1 v2 nil); intros Hpick.
+    elim Hpick; clear Hpick; intro v3; intros.
+    elim H2; clear H2; intros.
+    rewrite <- H2; clear H2.
+    destruct (equiv_dec v2 v3); try congruence; clear c.
+    simpl.
+    reflexivity.
+  Qed.
+
+  (** * Unnest *)
+  
+  Definition unnest_from_nraenv vid venv a b n1 := 
+    (NNRCFor (fresh_var "tmap$" (vid :: venv :: nil))
+             (NNRCUnop AFlatten
+                       (NNRCFor (fresh_var "tmc$" (vid :: venv :: nil))
+                                n1
+                                (NNRCFor
+                                   (fresh_var "tmc$" (fresh_var "tmc$" (vid :: venv :: nil) :: vid :: venv :: nil))
+                                   (NNRCFor (fresh_var "tmap$" (vid :: venv :: nil))
+                                            (NNRCUnop (ADot a) (NNRCVar (fresh_var "tmc$" (vid :: venv :: nil))))
+                                            (NNRCUnop (ARec b) (NNRCVar (fresh_var "tmap$" (vid :: venv :: nil)))))
+                                   (NNRCBinop AConcat (NNRCVar (fresh_var "tmc$" (vid :: venv :: nil)))
+                                              (NNRCVar
+                                                 (fresh_var "tmc$"
+                                                            (fresh_var "tmc$" (vid :: venv :: nil) :: vid :: venv :: nil)))))))
+             (NNRCUnop (ARecRemove a) (NNRCVar (fresh_var "tmap$" (vid :: venv :: nil))))).
+  
+  Definition unnest_from_nraenv_core vid venv a b n1 :=
+    (NNRCFor (fresh_var "tmap$" (vid :: venv :: nil))
+             (NNRCUnop AFlatten
+                       (NNRCFor (fresh_var "tmc$" (vid :: venv :: nil))
+                                n1
+                                (NNRCFor
+                                   (fresh_var "tmc$" (fresh_var "tmc$" (vid :: venv :: nil) :: vid :: venv :: nil))
+                                   (NNRCFor
+                                      (fresh_var "tmap$" (fresh_var "tmc$" (vid :: venv :: nil) :: venv :: nil))
+                                      (NNRCUnop (ADot a) (NNRCVar (fresh_var "tmc$" (vid :: venv :: nil))))
+                                      (NNRCUnop (ARec b)
+                                                (NNRCVar
+                                                   (fresh_var "tmap$"
+                                                              (fresh_var "tmc$" (vid :: venv :: nil) :: venv :: nil)))))
+                                   (NNRCBinop AConcat (NNRCVar (fresh_var "tmc$" (vid :: venv :: nil)))
+                                              (NNRCVar
+                                                 (fresh_var "tmc$"
+                                                            (fresh_var "tmc$" (vid :: venv :: nil) :: vid :: venv :: nil)))))))
+             (NNRCUnop (ARecRemove a) (NNRCVar (fresh_var "tmap$" (vid :: venv :: nil))))).
+
+  Lemma unnest_from_nraenv_and_nraenv_core_eq vid venv env a b op1 op1' :
+    nnrc_core_eval h env op1 = nnrc_core_eval h env op1' ->
+    nnrc_core_eval h env (unnest_from_nraenv vid venv a b op1) =
+    nnrc_core_eval h env (unnest_from_nraenv_core vid venv a b op1').
+  Proof.
+    intros Hind.
+    Opaque fresh_var.
+    simpl.
+    rewrite Hind; clear Hind.
+    destruct (nnrc_core_eval h env op1'); try reflexivity; simpl.
+    destruct d; try reflexivity; simpl.
+    destruct (equiv_dec (fresh_var "tmap$" (vid :: venv :: nil))
+                        (fresh_var "tmap$" (vid :: venv :: nil))); try congruence.
+    destruct (equiv_dec (fresh_var "tmc$" (vid :: venv :: nil))
+                        (fresh_var "tmc$" (vid :: venv :: nil))); try congruence.
+    simpl in *.
+    destruct (equiv_dec
+                (fresh_var "tmc$"
+                           (fresh_var "tmc$" (vid :: venv :: nil) :: vid :: venv :: nil))
+                (fresh_var "tmc$"
+                           (fresh_var "tmc$" (vid :: venv :: nil) :: vid :: venv :: nil)));
+      try congruence; simpl.
+    destruct (equiv_dec
+                (fresh_var "tmap$"
+                           (fresh_var "tmc$" (vid :: venv :: nil) :: venv :: nil))
+                (fresh_var "tmap$"
+                           (fresh_var "tmc$" (vid :: venv :: nil) :: venv :: nil))); try congruence; simpl in *.
+    destruct (equiv_dec (fresh_var "tmc$" (vid :: venv :: nil))
+                        (fresh_var "tmc$"
+                                   (fresh_var "tmc$" (vid :: venv :: nil)
+                                              :: vid :: venv :: nil))). auto.
+    clear e e0 e1 e2 c.
+    f_equal.
+    induction l; [reflexivity| ]; simpl.
+    destruct a0; try reflexivity.
+  Qed.
+  
+End NNRCSugar.
+
+(* 
+*** Local Variables: ***
+*** coq-load-path: (("../../../coq" "Qcert")) ***
+*** End: ***
+*)
